WIP: progress on updating the program logic for callbacks

theories/interop/wrapper_wp.v
@@ -50,7 +50,7 @@ Definition C_state_interp (ζ : lstore) (χ : lloc_map) (θ : addr_map) (roots :
   ∗ "SIχ" ∷ ghost_var wrapperGS_γχ (1/2) χ
   ∗ "SIθ" ∷ ghost_var wrapperGS_γθ (1/2) θ
   ∗ "SIroots" ∷ ghost_var wrapperGS_γroots_set (1/2) roots
-  ∗ "SIbound" ∷ ghost_var wrapperGS_γat_boundary (1/4) false.
+  ∗ "SIbound" ∷ ghost_var wrapperGS_γat_boundary (1/4) true.
 
 Definition GC (θ : addr_map) : iProp Σ :=
   ∃ (ζ ζfreeze ζσ ζvirt : lstore) (χ χvirt : lloc_map) (σMLvirt : store)
@@ -60,7 +60,7 @@ Definition GC (θ : addr_map) : iProp Σ :=
   ∗ "GCθ" ∷ ghost_var wrapperGS_γθ (1/2) θ
   ∗ "GCroots" ∷ ghost_var wrapperGS_γroots_set (1/2) roots_s
   ∗ "GCζvirt" ∷ lstore_own_auth wrapperGS_γζvirt ζvirt
-  ∗ "GCbound" ∷ ghost_var wrapperGS_γat_boundary (1/4) false
+  ∗ "GCbound" ∷ ghost_var wrapperGS_γat_boundary (1/4) true
   ∗ "(GCσMLv & GCnMLv & GCσdom)" ∷ state_interp σMLvirt nMLv
   ∗ "GCχvirt" ∷ lloc_own_auth wrapperGS_γχvirt χvirt
   ∗ "GCχNone" ∷ ([∗ map] _↦ℓ ∈ pub_locs_in_lstore χvirt ζvirt, ℓ ↦M/)
@@ -98,7 +98,7 @@ Definition ML_state_interp (ζvirt : lstore) (χ : lloc_map) (roots : roots_map)
   ∗ "SIχ" ∷ ghost_var wrapperGS_γχ (1/2) χ
   ∗ "SIθ" ∷ ghost_var wrapperGS_γθ (1/2) (∅ : addr_map)
   ∗ "SIroots" ∷ ghost_var wrapperGS_γroots_set (1/2) (dom roots)
-  ∗ "SIbound" ∷ ghost_var wrapperGS_γat_boundary (1/2) true
+  ∗ "SIbound" ∷ ghost_var wrapperGS_γat_boundary (1/2) false
   ∗ "SIζvirt" ∷ lstore_own_auth wrapperGS_γζvirt ζvirt
   ∗ "(HσCv & HnCv)" ∷ (state_interp (memC ∪ (fmap (fun k => None) roots)) nCv)
   ∗ "SIAχ" ∷ lloc_own_auth wrapperGS_γχvirt χ
@@ -108,17 +108,18 @@ Definition ML_state_interp (ζvirt : lstore) (χ : lloc_map) (roots : roots_map)
   ∗ "%Hother_blocks" ∷ ⌜dom ζvirt ⊆ dom χ⌝
   ∗ "%HmemCdisj" ∷ ⌜dom memC ## dom roots⌝.
 
-Definition public_state_interp : store -> iProp Σ := (λ σ, ∃ n, state_interp σ n)%I.
-Definition private_state_interp : wrapstateML -> iProp Σ := (λ ρml, ML_state_interp (ζML ρml) (χML ρml) (rootsML ρml) (privmemML ρml))%I.
+Definition public_state_interp : memory → iProp Σ := (λ mem, ∃ n, state_interp mem n)%I.
+Definition private_state_interp : wrapstateC → iProp Σ :=
+  (λ ρc, C_state_interp (ζC ρc) (χC ρc) (θC ρc) (rootsC ρc))%I.
 
 Definition wrap_state_interp (σ : Wrap.state) : iProp Σ :=
   match σ with
   | Wrap.CState ρc mem =>
-      "(%nCv & HσC & HnC)" ∷ (∃ n, state_interp mem n) ∗
-      "SIC"        ∷ C_state_interp (ζC ρc) (χC ρc) (θC ρc) (rootsC ρc)
+      "(%nCv & HσC & HnC)" ∷ public_state_interp mem ∗
+      "SIC"        ∷ private_state_interp ρc
   | Wrap.MLState ρml σ =>
-      "(%nMLv & HσML & HvML & HσMLdom)" ∷ public_state_interp σ ∗
-      "SIML"         ∷ private_state_interp ρml
+      "(%nMLv & HσML & HvML & HσMLdom)" ∷ (∃ n, state_interp σ n) ∗
+      "SIML"         ∷ ML_state_interp (ζML ρml) (χML ρml) (rootsML ρml) (privmemML ρml)
 end.
 
 Global Program Instance wrapGS :
@@ -137,16 +138,16 @@ Next Obligation.
   iIntros (σ pubσ privσ Hlink) "Hσ !>". inversion Hlink; subst. iApply "Hσ".
 Qed.
 Next Obligation.
-  iIntros (pubσ privσ) "Hpubσ Hprivσ !>".
-  iExists (MLState privσ pubσ). cbn. iSplitL; by iFrame.
+  iIntros (pubσ privσ) "Hpubσ Hprivσ !>". cbn.
+  iExists (CState privσ pubσ). cbn. iSplitL; by iFrame.
 Qed.
 Next Obligation.
   intros [ρc mem|ρml σ]; cbn; iIntros "Hb Hσ".
-  + iExists _, _. iPureIntro. econstructor.
   + iExFalso. iAssert (⌜true = false⌝)%I as "%Hdone".
     * iApply (ghost_var_agree with "Hb [Hσ]").
-      iNamed "Hσ". iNamed "SIC". iFrame.
+      iNamed "Hσ". iNamed "SIML". iFrame.
     * iPureIntro. congruence.
+  + iExists _, _. iPureIntro. econstructor.
 Qed.
 
 
@@ -154,20 +155,22 @@ Qed.
 Context (σ : Wrap.state).
 Notation SI := (weakestpre.state_interp σ).
 
-Notation "l ↦fresh{ dq } b" := (lstore_own_mut wrapperGS_γζvirt l dq (Mut, b) ∗ lloc_own_priv wrapperGS_γχvirt l)%I
+Notation "l ↦fresh{ dq } b" := (lstore_own_mut wrapperGS_γζvirt l dq (Bvblock (Mut, b)) ∗ lloc_own_priv wrapperGS_γχvirt l)%I
   (at level 20, format "l  ↦fresh{ dq }  b") : bi_scope.
 Notation "l ↦fresh b" := (l ↦fresh{DfracOwn 1} b)%I
   (at level 20, format "l  ↦fresh  b") : bi_scope.
-Notation "l ↦mut{ dq } b" := (lstore_own_mut wrapperGS_γζvirt l dq (Mut, b) ∗ ∃ ll, block_sim_raw ll l)%I
+Notation "l ↦mut{ dq } b" := (lstore_own_mut wrapperGS_γζvirt l dq (Bvblock (Mut, b)) ∗ ∃ ll, block_sim_raw ll l)%I
   (at level 20, format "l  ↦mut{ dq }  b") : bi_scope.
 Notation "l ↦mut b" := (l ↦mut{DfracOwn 1} b)%I
   (at level 20, format "l  ↦mut  b") : bi_scope.
-Notation "l ↦imm b" := (lstore_own_immut wrapperGS_γζvirt l (Immut, b))%I
+Notation "l ↦imm b" := (lstore_own_immut wrapperGS_γζvirt l (Bvblock (Immut, b)))%I
   (at level 20, format "l  ↦imm  b") : bi_scope.
 Notation "l ↦roots{ dq } w" := (l ↪[wrapperGS_γroots_map]{dq} w)%I
   (at level 20, format "l  ↦roots{ dq }  w") : bi_scope.
 Notation "l ↦roots w" := (l ↪[wrapperGS_γroots_map] w)%I
   (at level 20, format "l  ↦roots  w") : bi_scope.
+Notation "l ↦clos ( f , x , e )" := (lstore_own_immut wrapperGS_γζvirt l (Bclosure f x e))%I
+  (at level 20, format "l  ↦clos  ( f ,  x ,  e )").
 
 Fixpoint block_sim (v : MLval) (l : lval) : iProp Σ := match v with
   (ML_lang.LitV (ML_lang.LitInt x)) => ⌜l = (Lint x)⌝
@@ -177,7 +180,8 @@ Fixpoint block_sim (v : MLval) (l : lval) : iProp Σ := match v with
 | (ML_lang.PairV v1 v2) => ∃ γ lv1 lv2, ⌜l = (Lloc γ)⌝ ∗ γ ↦imm (TagDefault, [lv1;lv2]) ∗ block_sim v1 lv1 ∗ block_sim v2 lv2
 | (ML_lang.InjLV v) => ∃ γ lv, ⌜l = (Lloc γ)⌝ ∗ γ ↦imm (TagDefault, [lv]) ∗ block_sim v lv
 | (ML_lang.InjRV v) => ∃ γ lv, ⌜l = (Lloc γ)⌝ ∗ γ ↦imm (TagInjRV, [lv]) ∗ block_sim v lv 
-| (ML_lang.RecV _ _ _) => True end. (* TODO: callbacks ?? *)
+| (ML_lang.RecV f x e) => ∃ γ, ⌜l = Lloc γ⌝ ∗ γ ↦clos (f, x, e)
+ end.
 
 Global Instance block_sim_pers v l : Persistent (block_sim v l).
 Proof.
@@ -198,25 +202,25 @@ Qed.
 
 Lemma SI_not_at_boundary_is_in_ML :
   SI -∗ not_at_boundary -∗
-  ⌜∃ ρc mem, σ = CState ρc mem⌝.
+  ⌜∃ ρml s, σ = MLState ρml s⌝.
 Proof.
   iIntros "Hσ Hnb". destruct σ as [ρml σ' | ρc mem]; eauto.
-  iExFalso; iNamed "Hσ"; iNamed "SIML";
+  iExFalso. iNamed "Hσ"; iNamed "SIC".
   iPoseProof (ghost_var_agree with "Hnb SIbound") as "%HH"; congruence.
 Qed.
 
 End Embed_logic.
 
 (* reexport notations *)
-Notation "l ↦fresh{ dq } b" := (lstore_own_mut wrapperGS_γζvirt l dq (Mut, b) ∗ lloc_own_priv wrapperGS_γχvirt l)%I
+Notation "l ↦fresh{ dq } b" := (lstore_own_mut wrapperGS_γζvirt l dq (Bvblock (Mut, b)) ∗ lloc_own_priv wrapperGS_γχvirt l)%I
   (at level 20, format "l  ↦fresh{ dq }  b") : bi_scope.
 Notation "l ↦fresh b" := (l ↦fresh{DfracOwn 1} b)%I
   (at level 20, format "l  ↦fresh  b") : bi_scope.
-Notation "l ↦mut{ dq } b" := (lstore_own_mut wrapperGS_γζvirt l dq (Mut, b) ∗ ∃ ll, block_sim_raw ll l)%I
+Notation "l ↦mut{ dq } b" := (lstore_own_mut wrapperGS_γζvirt l dq (Bvblock (Mut, b)) ∗ ∃ ll, block_sim_raw ll l)%I
   (at level 20, format "l  ↦mut{ dq }  b") : bi_scope.
 Notation "l ↦mut b" := (l ↦mut{DfracOwn 1} b)%I
   (at level 20, format "l  ↦mut  b") : bi_scope.
-Notation "l ↦imm b" := (lstore_own_immut wrapperGS_γζvirt l (Immut, b))%I
+Notation "l ↦imm b" := (lstore_own_immut wrapperGS_γζvirt l (Bvblock (Immut, b)))%I
   (at level 20, format "l  ↦imm  b") : bi_scope.
 Notation "l ↦roots{ dq } w" := (l ↪[wrapperGS_γroots_map]{dq} w)%I
   (at level 20, format "l  ↦roots{ dq }  w") : bi_scope.
