theories/interop/wrapper_wp_utils.v
@@ -1,5 +1,5 @@
 From Coq Require Import ssreflect.
-From stdpp Require Import strings gmap.
+From stdpp Require Import strings gmap list.
 From melocoton Require Import named_props.
 From melocoton.mlanguage Require Import mlanguage.
 From melocoton.language Require Import language weakestpre.
@@ -76,12 +76,12 @@ Definition WP_modify_spec : spec := (λ n vl wp,
     "->" ∷ ⌜n = "modify"⌝ ∗
     "->" ∷ ⌜vl = [ w; C_lang.LitV $ C_lang.LitInt $ i; w' ]⌝ ∗
     "%Hreprw" ∷ ⌜repr_lval θ (Lloc γ) w⌝ ∗
-    "Hpto" ∷ lstore_own_mut wrapperGS_γζvirt γ (DfracOwn 1) (Mut, (tg, vs)) ∗
+    "Hpto" ∷ lstore_own_mut wrapperGS_γζvirt γ (DfracOwn 1) (Bvblock (Mut, (tg, vs))) ∗
     "%Hreprw'" ∷ ⌜repr_lval θ v' w'⌝ ∗
     "%Hi1" ∷ ⌜0 ≤ i⌝%Z ∗
     "%Hi2" ∷ ⌜i < length vs⌝%Z ∗
     "HWP" ∷ (GC θ -∗
-             lstore_own_mut wrapperGS_γζvirt γ (DfracOwn 1) (Mut, (tg, <[Z.to_nat i:=v']> vs)) -∗
+             lstore_own_mut wrapperGS_γζvirt γ (DfracOwn 1) (Bvblock (Mut, (tg, <[Z.to_nat i:=v']> vs))) -∗
              wp (C_lang.LitV $ C_lang.LitInt $ 0)))%I.
 
 (* The most general spec, prove stuff for specific block-level pointstos later *)
@@ -91,11 +91,11 @@ Definition WP_readfield_spec : spec := (λ n vl wp,
      "->" ∷ ⌜n = "readfield"⌝ ∗
      "->" ∷ ⌜vl = [ w; C_lang.LitV $ C_lang.LitInt $ i ]⌝ ∗
      "%Hreprw" ∷ ⌜repr_lval θ (Lloc γ) w⌝ ∗
-     "Hpto" ∷ lstore_own_elem wrapperGS_γζvirt γ dq (m, (tg, vs)) ∗
+     "Hpto" ∷ lstore_own_elem wrapperGS_γζvirt γ dq (Bvblock (m, (tg, vs))) ∗
      "%Hi1" ∷ ⌜0 ≤ i⌝%Z ∗
      "%Hi2" ∷ ⌜i < length vs⌝%Z ∗
      "HWP" ∷ (∀ v' w', GC θ -∗
-                       lstore_own_elem wrapperGS_γζvirt γ dq (m, (tg, vs)) -∗
+                       lstore_own_elem wrapperGS_γζvirt γ dq (Bvblock (m, (tg, vs))) -∗
                        ⌜vs !! (Z.to_nat i) = Some v'⌝ -∗
                        ⌜repr_lval θ v' w'⌝ -∗
                        wp w'))%I.
@@ -408,14 +408,15 @@ Lemma deserialize_ML_value χMLold v :
   ∧ is_val χC ζimm v lv.
 Proof.
   induction v as [[x|bo| |ℓ]| |v1 IHv1 v2 IHv2|v IHv|v IHv] in χMLold|-*; intros Hinj.
-  1-3,5: eexists χMLold, ∅, _; split_and!; [by eapply extended_to_refl | econstructor ].
-  Unshelve. 5: exact (Lloc 0). (* what happens for functions *)
+  1-3: eexists χMLold, ∅, _; split_and!; [by eapply extended_to_refl | econstructor ].
   - destruct (ensure_in_χ_pub χMLold ℓ) as (χ' & γ & Hχ' & Hγ & _); first done.
     exists χ', ∅, (Lloc γ); (split_and!; last by econstructor).
     by eapply extended_to_mono.
+  - destruct (allocate_in_χ_priv χMLold (Bclosure f x e)) as (χ & γ & Hextend); first done.
+    eexists _, _, (Lloc γ). split; eauto. econstructor. by simplify_map_eq.
   - destruct (IHv1 χMLold) as (χ1 & ζ1 & lv1 & Hext1 & Hlv1); first done.
     destruct (IHv2 χ1) as (χ2 & ζ2 & lv2 & Hext2 & Hlv2); first by eapply extended_to_inj.
-    pose (Immut,(TagDefault,[lv1;lv2])) as blk.
+    pose (Bvblock (Immut,(TagDefault,[lv1;lv2]))) as blk.
     edestruct (allocate_in_χ_priv χ2 blk) as (χ3 & γ & Hext3); first by eapply extended_to_inj.
     eassert (extended_to χMLold _ χ3).
     1: do 2 (eapply extended_to_trans; last done); done.
@@ -430,7 +431,7 @@ Proof.
       eapply is_val_mono; last done; try done.
       eapply map_union_subseteq_r. eapply extended_to_trans; done.
   - destruct (IHv χMLold) as (χ1 & ζ1 & lv1 & Hext1 & Hlv1); first done.
-    epose (Immut,(_,[lv1])) as blk.
+    epose (Bvblock (Immut,(_,[lv1]))) as blk.
     edestruct (allocate_in_χ_priv χ1 blk) as (χ3 & γ & Hext3); first by eapply extended_to_inj.
     eassert (extended_to χMLold _ χ3).
     1: (eapply extended_to_trans; last done); done.
@@ -441,7 +442,7 @@ Proof.
       apply lookup_singleton.
     + eapply is_val_extended_to_weaken; done.
   - destruct (IHv χMLold) as (χ1 & ζ1 & lv1 & Hext1 & Hlv1); first done.
-    epose (Immut,(_,[lv1])) as blk.
+    epose (Bvblock (Immut,(_,[lv1]))) as blk.
     edestruct (allocate_in_χ_priv χ1 blk) as (χ3 & γ & Hext3); first by eapply extended_to_inj.
     eassert (extended_to χMLold _ χ3).
     1: (eapply extended_to_trans; last done); done.
@@ -480,7 +481,7 @@ Lemma deserialize_ML_block χMLold vs :
 Proof.
   intros H.
   destruct (deserialize_ML_values χMLold vs H) as (χC & ζimm & lvs & H1 & H2).
-  by exists χC, ζimm, (Mut,(TagDefault,lvs)).
+  by exists χC, ζimm, (Bvblock (Mut,(TagDefault,lvs))).
 Qed.
 
 
@@ -677,43 +678,67 @@ End ChiZetaConstruction.
 
 Section ThetaConstruction.
 
-Lemma collect_dom_θ_vs (θdom : gset lloc) (vs : list lval) : exists θdom' : gset lloc, forall γ, (Lloc γ ∈ vs ∨ γ ∈ θdom) ↔ γ ∈ θdom'.
+Lemma collect_dom_θ_vs (θdom : gset lloc) (vs : list lval) :
+  exists θdom' : gset lloc,
+    ∀ γ, Lloc γ ∈ vs ∨ γ ∈ θdom ↔ γ ∈ θdom'.
 Proof.
   induction vs as [|[|ℓ] vs (θdom1 & IH)].
-  - exists θdom. intros γ. split; last eauto. intros [[]%not_elem_of_nil|?]; done.
-  - exists θdom1. intros γ. split.
-    + intros [[Hc|H]%elem_of_cons|?]; try congruence; apply IH. 1: by left. by right.
-    + intros [H|H]%IH; last by right. left. right. done.
+  - exists θdom. intros γ. split; last eauto. by intros [H%elem_of_nil|].
+  - exists θdom1. intros γ. etransitivity; last by eapply IH.
+    split; (intros [H|]; last by eauto); left.
+    + apply elem_of_cons in H as [|]; done.
+    + apply elem_of_cons; eauto.
   - exists (θdom1 ∪ {[ ℓ ]}). intros γ. split.
-    + intros [[Hc|H]%elem_of_cons|?]; eapply elem_of_union. 1: right; eapply elem_of_singleton; congruence.
+    + intros [[Hc|H]%elem_of_cons|?]; eapply elem_of_union.
+      1: right; eapply elem_of_singleton; congruence.
       all: left; apply IH. 1: by left. by right.
-    + intros [[H|H]%IH| ->%elem_of_singleton]%elem_of_union. 1: left; right; done. 1: right; done.    
-      left; left; done.
+    + intros [[H|H]%IH| ->%elem_of_singleton]%elem_of_union.
+      1: left; by right. 1: by right.
+      left; by left.
 Qed.
 
-Lemma collect_dom_θ_ζ_blocks (θdom : gset lloc) (ζ : lstore) : exists θdom' : gset lloc,
-    forall γ, ((exists γ1 m t vs, ζ !! γ1 = Some (m, (t, vs)) ∧ Lloc γ ∈ vs) ∨ γ ∈ θdom) ↔ γ ∈ θdom'.
+Lemma collect_dom_θ_block (θdom : gset lloc) (blk : block) :
+  exists θdom' : gset lloc,
+    ∀ γ, lval_in_block blk (Lloc γ) ∨ γ ∈ θdom ↔ γ ∈ θdom'.
 Proof.
-  induction ζ as [|k [m [t vs]] ζ Hne (θdom1 & Hdom1)] using map_ind.
-  - exists θdom; split.
-    + intros [(γ1&m&t&vs&H1&H2)|Hold]; last done.
-      rewrite lookup_empty in H1; done.
-    + intros H; by right.
-  - destruct (collect_dom_θ_vs θdom1 vs) as (θdom2 & Hdom2).
+  destruct blk as [[m [tg vs]]|]; last first.
+  { (* Bclosure *)
+    exists θdom. intros γ. split; eauto. intros [H|]; auto.
+    by inversion H. }
+  { (* Bvblock *)
+    destruct (collect_dom_θ_vs θdom vs) as (θdom' & H).
+    exists θdom'. intros γ. split.
+    - intros [HH|]; first inversion HH; subst; apply H; eauto.
+    - intros [?|?]%H; eauto. left; by constructor. }
+Qed.
+
+Lemma collect_dom_θ_ζ_blocks (θdom : gset lloc) (ζ : lstore) :
+  exists θdom' : gset lloc,
+    forall γ, ((exists γ1 blk, ζ !! γ1 = Some blk ∧ lval_in_block blk (Lloc γ))
+               ∨ γ ∈ θdom)
+              ↔ γ ∈ θdom'.
+Proof.
+  induction ζ as [|k blk ζ Hne (θdom1 & Hdom1)] using map_ind.
+  - exists θdom; split; auto. intros [(γ1&blk&H1&_)|]; auto.
+    simplify_map_eq.
+  - destruct (collect_dom_θ_block θdom1 blk) as (θdom2 & Hdom2).
     exists θdom2. intros γ; split.
-    + intros [(γ1&m'&t'&vs'&[[-> Hinj]|[Hne2 Hin]]%lookup_insert_Some&H2)|Hold].
-      1: apply Hdom2; left; congruence.
-      1: apply Hdom2; right; apply Hdom1; left; by repeat eexists.
-      1: apply Hdom2; right; apply Hdom1; right; done.
-    + intros [H|[(γ1&m'&t'&vs'&H1&H2)|H]%Hdom1]%Hdom2.
-      1: left; do 4 eexists; split; first eapply lookup_insert; done.
+    + intros [(γ1&blk'&[[-> ->]|[Hne2 Hin]]%lookup_insert_Some&H2)|Hold].
+      { apply Hdom2; left; congruence. }
+      { apply Hdom2. right. apply Hdom1. left. by do 2 eexists. }
+      { apply Hdom2; right; apply Hdom1; right; done. }
+    + intros [H|[(γ1&blk'&H1&H2)|H]%Hdom1]%Hdom2.
+      1: left; do 2 eexists; split; first eapply lookup_insert; done.
       2: by right.
-      left; do 4 eexists; split; last done; first rewrite lookup_insert_ne; first done.
+      left; do 2 eexists; split; last done; first rewrite lookup_insert_ne; first done.
       intros ->; rewrite Hne in H1; congruence.
 Qed.
 
-Lemma collect_dom_θ_ζ (θdom : gset lloc) (ζ : lstore) : exists θdom' : gset lloc,
-    forall γ, (γ ∈ dom ζ ∨ (exists γ1 m t vs, ζ !! γ1 = Some (m, (t, vs)) ∧ Lloc γ ∈ vs) ∨ γ ∈ θdom) ↔ γ ∈ θdom'.
+Lemma collect_dom_θ_ζ (θdom : gset lloc) (ζ : lstore) :
+  exists θdom' : gset lloc,
+    forall γ, (γ ∈ dom ζ ∨ (exists γ1 blk, ζ !! γ1 = Some blk ∧ lval_in_block blk (Lloc γ))
+               ∨ γ ∈ θdom)
+              ↔ γ ∈ θdom'.
 Proof.
   destruct (collect_dom_θ_ζ_blocks θdom ζ) as (θdom1 & Hdom1).
   exists (dom ζ ∪ θdom1). intros γ; split.
@@ -842,7 +867,7 @@ Proof.
   destruct (find_repr_roots θC (rootsML ρml) (privmemML ρml)) as (mem & Hrepr); [done..|].
 
   eexists ws, (WrapstateC χ2 ζC θC _), mem. unfold ml_to_c; cbn.
-  exists ζσ, (ζσimm ∪ ζimm), lvs. split_and!.
+  exists ζσ, (ζσimm ∪ ζimm), lvs. split_and!; try done.
   { eapply extended_to_trans; done. }
   { destruct Hstorebl as [HL HR]; split.
     { intros ℓ  Hℓ. destruct (HL ℓ Hℓ) as (γ & Hγ). exists γ. eapply lookup_weaken; first done. apply Hext2. }
@@ -852,7 +877,6 @@ Proof.
        enough (γ2 = γ) as -> by done. eapply Hext2. 2: done. eapply lookup_weaken; first done; eapply Hext2. } }
   { intros γ. rewrite dom_union_L. intros [H|H]%elem_of_union; eapply lookup_weaken.
     1: by eapply Hext. 2: by eapply Hext2. 2: done. 1: apply Hext2. }
-  { reflexivity. }
   { rewrite map_union_assoc. apply map_disjoint_union_r_2. 1: done.
     eapply map_disjoint_dom, disjoint_weaken; first eapply map_disjoint_dom, Hdis1; try done.
     erewrite ! dom_union_L; set_solver. }
@@ -866,12 +890,8 @@ Proof.
     + eapply map_union_subseteq_l. }
   { eapply Forall2_impl; first done. intros ? ? H; eapply is_val_mono; last done; first done.
     unfold ζC. rewrite ! map_union_assoc. eapply map_union_subseteq_r. done. }
-  { split; first done. subst θdom3. intros γ m tg vs' γ' _ H2 H3.
-    apply Hθdom3. right. apply Hθdom2. right. apply Hθdom1. right. left. do 4 eexists; done. }
-  { done. }
-  { done. }
-  { done. }
-  { done. }
+  { split; first done. subst θdom3. intros γ blk γ' _ H2 H3.
+    apply Hθdom3. right. apply Hθdom2. right. apply Hθdom1. right. left. do 2 eexists; done. }
 Qed.
 
 End Utils.
